Completed the proof.

Casper.thy
@@ -1,13 +1,11 @@
 theory Casper
-imports Main "Eisbach"
+imports Main "HOL-Eisbach.Eisbach" Inductive
 begin
 
 locale byz_quorums =
   fixes member_1 :: "'n \<Rightarrow> 'q1 \<Rightarrow> bool" (infix "\<in>\<^sub>1" 50)(* membership in 2/3 set *)
     and member_2 :: "'n \<Rightarrow> 'q2 \<Rightarrow> bool" (infix "\<in>\<^sub>2" 50)(* membership in 1/3 set *)
   assumes "\<And> q1 q2 . \<exists> q3 . \<forall> n . n \<in>\<^sub>2 q3 \<longrightarrow> n \<in>\<^sub>1 q1 \<and> n \<in>\<^sub>1 q2"  (* 2/3 quorums have 1/3 intersection *)
-    (* and "\<And> q1 q2 . \<exists> n . n \<in>\<^sub>2 q1 \<and> n \<in>\<^sub>1 q2" *) (* 2/3 sets and 1/3 sets intersect *)
-    (* and "\<And> q . \<exists> n . n \<in>\<^sub>2 q" *)
 
 record ('n,'h,'v)state =
   -- "@{typ 'n} is the type of validators (nodes), @{typ 'h} hashes, and @{typ nat} views"
@@ -16,7 +14,7 @@ record ('n,'h,'v)state =
 
 locale casper = byz_quorums +
 fixes 
-  hash_pred :: "'h \<Rightarrow> 'h \<Rightarrow> bool" (infix "\<leftarrow>" 50)
+  hash_parent :: "'h \<Rightarrow> 'h \<Rightarrow> bool" (infix "\<leftarrow>" 50)
 assumes
   -- "a hash has at most one predecessor which is not itself"
   "\<And> h1 h2 . h1 \<leftarrow> h2 \<Longrightarrow> h1 \<noteq> h2"
@@ -27,37 +25,51 @@ inductive hash_ancestor (infix "\<leftarrow>\<^sup>*" 50) where
   "h1 \<leftarrow> h2 \<Longrightarrow> h1 \<leftarrow>\<^sup>* h2"
 | "\<lbrakk>h1 \<leftarrow> h2; h2 \<leftarrow>\<^sup>* h3\<rbrakk> \<Longrightarrow> h1 \<leftarrow>\<^sup>* h3"
 declare hash_ancestor.intros[simp,intro]
+lemma hash_ancestor_intro': assumes "h1 \<leftarrow>\<^sup>* h2" and "h2 \<leftarrow> h3" shows "h1 \<leftarrow>\<^sup>* h3" using assms
+  by (induct h1 h2 rule:hash_ancestor.induct) auto
 
-inductive nth_parent :: "nat \<Rightarrow> 'h \<Rightarrow> 'h \<Rightarrow> bool" where 
-  "nth_parent 0 h1 h1"
-| "\<lbrakk>nth_parent n h1 h2; h2 \<leftarrow> h3\<rbrakk> \<Longrightarrow> nth_parent (n+1) h1 h3"
-declare nth_parent.intros[simp,intro]
+inductive nth_ancestor :: "nat \<Rightarrow> 'h \<Rightarrow> 'h \<Rightarrow> bool" where 
+  "nth_ancestor 0 h1 h1"
+| "\<lbrakk>nth_ancestor n h1 h2; h2 \<leftarrow> h3\<rbrakk> \<Longrightarrow> nth_ancestor (n+1) h1 h3"
+declare nth_ancestor.intros[simp,intro]
 
-inductive_cases test2:"nth_parent 1 h1 h2"
-thm test2
+inductive_cases nth_ancestor_succ:"nth_ancestor (n+1) h1 h3"
+inductive_cases zeroth_ancestor:"nth_ancestor 0 h1 h3"
 
-lemmas casper_assms_def = casper_def casper_axioms_def class.linorder_def class.order_def
-    class.preorder_def class.order_axioms_def class.linorder_axioms_def byz_quorums_def
-    class.order_bot_def class.order_bot_axioms_def
+lemma parent_ancestor:"h1 \<leftarrow> h2 = nth_ancestor 1 h1 h2"
+  by (metis One_nat_def add.right_neutral add_Suc_right add_diff_cancel_left' diff_Suc_Suc nat.simps(3) nth_ancestor.simps)
 
-text {* All messages in epoch @{term 0} are ignored;  @{term 0} is used as a special value. *}
+lemma "\<lbrakk>nth_ancestor (n+1) h1 h2; h3 \<leftarrow> h2\<rbrakk> \<Longrightarrow> nth_ancestor n h1 h3"
+  by (metis casper.axioms(2) casper_axioms casper_axioms_def nth_ancestor_succ)
+  
+lemmas casper_assms_def = casper_def casper_axioms_def byz_quorums_def
 
-definition prepared where 
-  "prepared s q h v1 v2 \<equiv> v1 \<noteq> 0 \<and> (\<forall> n . n \<in>\<^sub>1 q \<longrightarrow> prepare_msg s n h v1 v2)"
+lemma "h1 \<leftarrow>\<^sup>* h2 \<Longrightarrow> \<not> h2 \<leftarrow>\<^sup>* h1" 
+  nitpick[no_assms,verbose, card 'h=2, eval="(op \<leftarrow>,UNIV::'h set)"]
+    -- "The definition allows loops."
+  oops
+
+  text {* All messages in epoch @{term 0} are ignored;  @{term 0} is used as a special value. 
+  This appears in the following definitions. *}
+
+definition prepared' where
+  "prepared' s q h v1 v2 \<equiv> v1 \<noteq> 0 \<and> (\<forall> n . n \<in>\<^sub>1 q \<longrightarrow> prepare_msg s n h v1 v2)"
+definition prepared where
+  "prepared s q h v1 v2 \<equiv> v1 \<noteq> 0 \<and> v2 < v1 \<and> (\<forall> n . n \<in>\<^sub>1 q \<longrightarrow> prepare_msg s n h v1 v2)"
 definition committed where
   "committed s q h v \<equiv> v \<noteq> 0 \<and> (\<forall> n . n \<in>\<^sub>1 q \<longrightarrow> commit_msg s n h v)"
 definition fork where 
   "fork s \<equiv> \<exists> h1 h2 q1 q2 v1 v2 . committed s q1 h1 v1 \<and> committed s q2 h2 v2
     \<and> \<not>(h2 \<leftarrow>\<^sup>* h1 \<or> h1 \<leftarrow>\<^sup>* h2 \<or> h1 = h2)"
 
-definition slashed_1 where  "slashed_1 s n \<equiv> 
+definition slashed_1 where  "slashed_1 s n \<equiv>
   \<exists> h v . commit_msg s n h v \<and> (\<forall> q v2 . v2 < v \<longrightarrow> \<not>prepared s q h v v2)"
 definition slashed_2 where
   "slashed_2 s n \<equiv>
   \<exists> h v1 v2 . prepare_msg s n h v1 v2 \<and> v2 \<noteq> 0 \<and>
-    (\<forall> v3 q h2 . v3 < v2 \<longrightarrow> \<not>(nth_parent (v1 - v2) h2 h \<and> prepared s q h2 v2 v3))"
+    (\<forall> v3 q h2 . v3 < v2 \<longrightarrow> \<not>(nth_ancestor (v1 - v2) h2 h \<and> prepared s q h2 v2 v3))"
 definition slashed_2' where
-  -- "this is not exactly what Vitalik wrote."
+  -- "this is not what Vitalik wrote, but works too."
   "slashed_2' s n \<equiv>
   \<exists> h v1 v2 . prepare_msg s n h v1 v2 \<and> v2 \<noteq> 0 \<and>
     (\<forall> v3 q h2 . v3 < v2 \<longrightarrow> \<not>(h2 \<leftarrow> h \<and> prepared s q h2 v2 v3))"
@@ -68,48 +80,111 @@ definition slashed_3 where
 definition slashed_4 where
   "slashed_4 s n \<equiv> \<exists> h1 h2 v v1 v2 . (h1 \<noteq> h2 \<or> v1 \<noteq> v2) \<and> 
     prepare_msg s n h1 v v1 \<and> prepare_msg s n h2 v v2"
-
 definition slashed where "slashed s n \<equiv> 
   slashed_1 s n \<or> slashed_2 s n \<or> slashed_3 s n \<or> slashed_4 s n"
+definition one_third_slashed where "one_third_slashed s \<equiv> \<exists> q . \<forall> n . n \<in>\<^sub>2 q \<longrightarrow> slashed s n"
+lemmas slashed_defs = slashed_def slashed_1_def slashed_2_def slashed_4_def slashed_3_def one_third_slashed_def
 
-lemma assumes "prepared s q h1 v1 v2" and "committed s q h2 v2" and "v1 > v2"
-  and "\<not>nth_parent (v1 - v2) h2 h1"
-shows "\<exists> q . \<forall> n . n \<in>\<^sub>2 q \<longrightarrow> slashed s n"
-  using assms
-proof (induct "v1 - v2 - 1")
+lemmas order_defs = class.linorder_axioms_def class.linorder_def class.order_def class.preorder_def class.order_axioms_def class.order_bot_def class.order_bot_axioms_def linorder_axioms[where ?'a=nat]
+lemmas casper_defs = slashed_defs prepared_def fork_def committed_def casper_assms_def
+
+lemma assumes "\<not>one_third_slashed s" and "committed s q1 h1 v1" and "committed s q2 h2 v2"
+  and "h1 \<leftarrow>\<^sup>* h2" and "h2 \<leftarrow>\<^sup>* h1" shows False
+  nitpick[verbose, card 'b=1, card 'c=1, card 'a=1, card nat=3, card 'h=2, card 'd=1,
+      card "('a, 'h, nat, 'd) state_scheme" = 1, dont_box, timeout=300, eval="(\<lambda> h v1 v2 . \<exists> q . prepared s q h v1 v2)"]
+  -- "The slashing conditions allow loops in the block chain."
+  oops
+
+lemma assumes "\<not>one_third_slashed s" and "committed s q h v"
+  obtains q0 h0 v0 where "prepared s q0 h0 1 v0"
+  nitpick[verbose, card 'b=1, card 'c=1, card 'a=1, card nat=3, card 'h=2, card 'd=1,
+      card "('a, 'h, nat, 'd) state_scheme" = 1, dont_box, timeout=300, eval="fork s"]
+  -- "The slashing conditions allow a chain not anchored at 0."
+  oops
+
+lemma l1: assumes "prepared s q1 h1 v1 v2" and "committed s q2 h2 v3" and "v1 > v3" and "\<not>one_third_slashed s"
+  shows "v1 > v2 \<and> v2 \<ge> v3"
+  nitpick[verbose, card 'b=1, card 'c=1, card 'a=1, card nat=5, card 'h=4, card 'd=1,
+      card "('a, 'h, nat, 'd) state_scheme" = 1, dont_box, timeout=300, eval="fork s"]
+  using assms casper_axioms linorder_axioms[where ?'a=nat]
+  unfolding casper_defs order_defs
+  by smt
+
+lemma l2: assumes "nth_ancestor n h1 h2" and "nth_ancestor m h2 h3" 
+  shows "nth_ancestor (n+m) h1 h3" 
+  using assms 
+proof (induct m arbitrary: h1 h2 h3)
   case 0
-  have "\<not>h2 \<leftarrow> h1"
-    by (metis "0.hyps" Nat.add_0_right One_nat_def Suc_diff_Suc add_Suc_right assms(3) assms(4) diff_diff_left nth_parent.intros(1) nth_parent.intros(2))  
-  then show ?case using 0
-  using assms casper_axioms nth_parent.intros
-  unfolding slashed_def slashed_1_def slashed_2_def slashed_4_def slashed_3_def
-      prepared_def fork_def committed_def casper_assms_def
-  apply auto
-  using [[smt_infer_triggers,smt_timeout=3000,smt_oracle=true,smt_random_seed=3143,smt_certificates="./casper.cert"]]
+  then show ?case using nth_ancestor.cases by auto
 next
-  case (Suc x)
-  then show ?case sorry
-qed oops
+  case (Suc m)
+  then show ?case
+    by (metis Suc_eq_plus1 add_Suc_right nth_ancestor.simps nth_ancestor_succ)
+qed
 
-lemma assumes "fork s"
-  shows "\<exists> q . \<forall> n . n \<in>\<^sub>2 q \<longrightarrow> slashed s n" oops
-  using [[]]
-  nitpick[verbose, card 'b=2, card 'c=2, card 'a=5, card nat=5, card 'h=4, card 'd=1,
-      card "('a, 'h, nat, 'd) state_scheme" = 1, dont_box, timeout=300] (*,
-      eval="(slashed s, committed s)"] *)
-  using assms casper_axioms
-  apply -
-  unfolding slashed_def slashed_1_def slashed_2_def slashed_4_def slashed_3_def
-      prepared_def fork_def committed_def
-  apply (cases s)
-  apply simp
-  using hash_ancestor.intros nth_parent.intros
-  unfolding casper_assms_def
-  apply (simp (no_asm_use))
-  apply (match premises in P[thin]:"?x = ?y" \<Rightarrow> \<open>-\<close>)
-  apply clarify oops
-  using [[smt_infer_triggers,smt_timeout=3000,smt_oracle=true,smt_random_seed=8789797972,smt_certificates="./casper.cert"]]
-  sledgehammer[timeout=5000, provers=z3 spass]()
+lemma l3: assumes "prepared s q1 h1 v1 v2" and "committed s q2 h2 v3" and "v1 > v3" and "\<not>one_third_slashed s"
+  shows "nth_ancestor (v1 - v3) h2 h1"
+  nitpick[verbose, card 'b=1, card 'c=1, card 'a=1, card nat=5, card 'h=4, card 'd=1,
+      card "('a, 'h, nat, 'd) state_scheme" = 1, dont_box, timeout=300, eval="fork s"]
+proof -
+  show ?thesis using assms
+  proof (induct "v1 - v3" arbitrary: v1 v2 v3 q1 q2 h1 h2 rule:less_induct)
+    case less
+    then show ?case 
+    proof (cases "v1-v3=0")
+      case True
+      then show ?thesis
+        using less.prems(3) by linarith 
+    next
+      case False
+      then show ?thesis
+      proof (cases "v2=v3")
+        case True
+        then show ?thesis using less(2-5) casper_axioms linorder_axioms[where ?'a=nat]
+          using [[smt_solver=cvc4]] by (simp add: casper_defs, unfold order_defs) smt
+      next
+        case False
+        obtain q3 h3 v4 where 1:"nth_ancestor (v1-v2) h3 h1" and 2:"prepared s q3 h3 v2 v4"
+          by (metis less.prems(1-3) assms(4) byz_quorums_axioms byz_quorums_def committed_def diff_is_0_eq diff_zero l1 one_third_slashed_def prepared_def slashed_2_def slashed_def)
+        have 3:"nth_ancestor (v2-v3) h2 h3"
+          by (metis False 2 l1 diff_less_mono less.hyps less.prems less_le)
+        have 4:"v1 > v2 \<and> v2 \<ge> v3" using assms casper.l1 casper_axioms less.prems(1-3) by metis
+        show ?thesis using 1 3 4 less.prems(3) l2 by force
+      qed
+    qed
+  qed
+qed
 
+lemma l4:assumes "nth_ancestor n (h1::'h) h2"
+  shows "h1 \<leftarrow>\<^sup>* h2 \<or> h1 = h2"
+  using assms
+proof (induct n arbitrary:h1 h2)
+  case 0
+  then show ?case using zeroth_ancestor by auto
+next
+  case (Suc n)
+  obtain h3 where 1:"h3 \<leftarrow> h2" and 2:"nth_ancestor n h1 h3" using nth_ancestor_succ Suc.prems by (metis Suc_eq_plus1) 
+  show ?case using Suc.hyps[OF 2] 1 hash_ancestor_intro' by blast 
+qed
+
+lemma safety: assumes "fork s" shows "one_third_slashed s"
+proof -
+  obtain h1 h2 q1 q2 v1 v2 where 1:"committed s q1 h1 v1" and 2:"committed s q2 h2 v2" 
+    and 3:"\<not> (h2 \<leftarrow>\<^sup>* h1 \<or> h1 \<leftarrow>\<^sup>* h2 \<or> h1 = h2)" using assms fork_def by blast
+  have 4:"\<not>(nth_ancestor n h1 h2 \<or> nth_ancestor n h2 h1 \<or> h1 = h2)" for n using l4 3 by auto
+  obtain q3 q4 v3 v4 where 5:"prepared s q3 h1 v1 v3" and 6:"prepared s q4 h2 v2 v4" if "\<not>one_third_slashed s" using 1 2
+    by (metis byz_quorums_axioms byz_quorums_def committed_def one_third_slashed_def slashed_1_def slashed_def)
+  show ?thesis 
+  proof (cases "v1 = v2")
+    case True
+    show ?thesis using 1 4 2 5 6 True casper_axioms unfolding byz_quorums_def casper_def
+      one_third_slashed_def casper_axioms committed_def prepared_def slashed_1_def slashed_4_def slashed_def
+      by metis
+  next
+    case False
+    thus ?thesis using l3 1 2 4 5 6
+      by (metis less_le not_less)
+  qed
+qed
 
 end
